extract/PatternImports.ml
@@ -4,3 +4,4 @@ open Term
 open Monads
 open List0 (*fold_left*)
 open Datatypes (*app*)
+open CoqUtil
