extract/ty.mli
@@ -201,3 +201,7 @@ val oty_cons : ty list -> ty option -> ty list
 val oty_match : ty Mtv.t -> ty option -> ty option -> ty Mtv.t
 val oty_inst  : ty Mtv.t -> ty option -> ty option
 val oty_freevars : Stv.t -> ty option -> Stv.t
+
+(*unsafe - for internal use only*)
+val ty_inst_unsafe  : ty Mtv.t -> ty -> ty
+val ty_match_aux : ty Mtv.t -> ty -> ty -> ty Mtv.t
