src/core/PatternComp.v
@@ -3,8 +3,33 @@ Require Import TermDefs TermFuncs Monads.
 Require CoqBigInt.
 Import MonadNotations.
 Require Import PatternAux.
+(* Require Import TaskDefs (*For hashcons full - TODO: move*). *)
 
 Local Open Scope err_scope.
+
+(*TODO: move*)
+Fixpoint rev_map_aux {A B: Type} (f: A -> B) accu l:=
+  match l with
+  | [] => accu
+  | a :: l => rev_map_aux f (f a :: accu) l
+  end.
+
+Definition rev_map {A B: Type} (f: A -> B) (l: list A) : list B :=
+  rev_map_aux f nil l.
+
+Lemma rev_map_aux_eq {C D: Type} (f: C -> D) accu (l: list C):
+  rev_map_aux f accu l = (map f (rev l)) ++ accu.
+Proof.
+  revert accu.
+  induction l as [| h t IH]; simpl; auto; intros accu.
+  rewrite IH, map_app. simpl. rewrite <- app_assoc. reflexivity.
+Qed.
+
+Lemma rev_map_eq {C D: Type} (f: C -> D) (l: list C):
+  rev_map f l = map f (rev l).
+Proof.
+  unfold rev_map. rewrite rev_map_aux_eq, app_nil_r. reflexivity.
+Qed.
 
 Definition NonExhaustive (l: list pattern_c) : errtype := 
   mk_errtype "NonExhaustive" l.
@@ -58,20 +83,26 @@ Fixpoint populate
       foldl_err populate rl (Mls.empty, nil).
 End Populate.
 
+Local Open Scope errst_scope.
+
+(*TODO: move*)
+Notation errst_throw e := (errst_lift2 (throw e)).
+
 Section Dispatch.
-Context {A B: Type} (mk_let: vsymbol -> term_c -> B -> B) (t: term_c) 
+(*mk_let can be [t_let_close_simp], which uses [t_subst], which is stateful*)
+Context {A: Type} (mk_let: vsymbol -> term_c -> A -> errState CoqBigInt.t A) (t: term_c) 
   (types: Mls.t (list pattern_c)).
 
 (*For dispatch, we need Equations, since it is not structurally recursive*)
-Definition add_case (fs: lsymbol) (pl: list pattern_c) (a: B) cases :=
+Definition add_case (fs: lsymbol) (pl: list pattern_c) (a: A) cases :=
     Mls.change _ (fun x =>
       match x with
       | None => Some [(pl, a)]
       | Some rl => Some ((pl, a) :: rl)
       end) fs cases.
 
-Definition union_cases pl (a: B) (types : Mls.t (list pattern_c)) cases :
-    Mls.t (list (list pattern_c * B)) :=
+Definition union_cases pl (a: A) (types : Mls.t (list pattern_c)) cases :
+    Mls.t (list (list pattern_c * A)) :=
     let add pl q := pat_wild (pat_ty_of q) :: pl in
     let wild ql := [(fold_left add ql pl, a)] in
     let join _ wl rl := Some (wl ++ rl) in
@@ -108,83 +139,45 @@ Qed.
 (*TODO: really termination metric is just size of first elt of list*)
 (*NOTE: [pat_node_of] makes this VERY annoying*)
 (*TODO: rewrite with Equations, generates LOTS of unhelpful stuff*)
-Fixpoint dispatch_aux (pla: list pattern_c * B) 
-  (casewild: (Mls.t (list (list pattern_c * B)) * list (list pattern_c * B)))
+Fixpoint dispatch_aux (pla: list pattern_c * A) 
+  (casewild: (Mls.t (list (list pattern_c * A)) * list (list pattern_c * A)))
   (ACC: Acc lt (list_pattern_c_size (fst pla))) :
-    errorM (Mls.t (list (list pattern_c * B)) * list (list pattern_c * B)) :=
+    errState CoqBigInt.t (Mls.t (list (list pattern_c * A)) * list (list pattern_c * A)) :=
     let cases := fst casewild in
     let wilds := snd casewild in
     match (fst pla) as o return o = fst pla -> _ with
-    | nil => fun _ => throw (Failure "hd")
+    | nil => fun _ => errst_throw (Failure "hd")
     | p :: pl => fun Hpl =>
       let cases := fst casewild in
       let wilds := snd casewild in
       let a := snd pla in
       match (pat_node_of p) as p' return pat_node_of p = p' -> _ with
       | Papp fs pl' => fun Heq =>
-        err_ret (add_case fs (rev_append pl' pl) a cases, wilds)
-      | Pwild => fun Heq => err_ret (union_cases pl a types cases, (pl, a) :: wilds)
+        errst_ret (add_case fs (rev_append pl' pl) a cases, wilds)
+      | Pwild => fun Heq => errst_ret (union_cases pl a types cases, (pl, a) :: wilds)
       | Por p1 q1 => fun Heq =>
         d1 <- dispatch_aux (q1 :: pl, a) (cases, wilds) (Acc_inv ACC (dispatch_aux_or2 Hpl Heq)) ;;
         dispatch_aux (p1 :: pl, a) d1 (Acc_inv ACC (dispatch_aux_or1 Hpl Heq))
       | Pas p x => fun Heq =>
-        dispatch_aux (p :: pl, mk_let x t a) (cases,wilds) (Acc_inv ACC (dispatch_aux_bind Hpl Heq))
+        a <- mk_let x t a ;;
+        dispatch_aux (p :: pl, a) (cases,wilds) (Acc_inv ACC (dispatch_aux_bind Hpl Heq))
       | Pvar x => fun Heq =>
-        let a := mk_let x t a in
-        err_ret (union_cases pl a types cases, (pl, a) :: wilds) 
+        a <- mk_let x t a ;;
+        errst_ret (union_cases pl a types cases, (pl, a) :: wilds) 
       end eq_refl
     end eq_refl.
 
-Definition dispatch_aux' (pla: list pattern_c * B) 
-  (casewild: (Mls.t (list (list pattern_c * B)) * list (list pattern_c * B))) :
-    errorM (Mls.t (list (list pattern_c * B)) * list (list pattern_c * B)) :=
+Definition dispatch_aux' (pla: list pattern_c * A) 
+  (casewild: (Mls.t (list (list pattern_c * A)) * list (list pattern_c * A))) :
+    errState CoqBigInt.t (Mls.t (list (list pattern_c * A)) * list (list pattern_c * A)) :=
   dispatch_aux pla casewild (Wf_nat.lt_wf _).
 
-
-(* 
-
-Equations dispatch_aux (pla: list pattern_c * B) 
-  (casewild: (Mls.t (list (list pattern_c * B)) * list (list pattern_c * B))) :
-    errorM (Mls.t (list (list pattern_c * B)) * list (list pattern_c * B))
-  by wf (list_pattern_c_size (fst pla)) lt:=
-  dispatch_aux (p :: pl, a) (cases, wilds) :=
-  (* let cases := fst casewild in
-  let wilds := snd casewild in
-  let a := snd pla in
-  p <- hd (fst pla) ;;
-  pl <- tl (fst pla) ;; *)
-    match (pat_node_of p) as p' return pat_node_of p = p' -> _ with
-    | Papp fs pl' => fun Heq =>
-      err_ret (add_case fs (rev_append pl' pl) a cases, wilds)
-    | Pwild => fun Heq => err_ret (union_cases pl a types cases, (pl, a) :: wilds)
-    | Por p1 q1 => fun Heq =>
-      d1 <- dispatch_aux (q1 :: pl, a) (cases, wilds) ;;
-      dispatch_aux (p1 :: pl, a) d1
-    | Pas p x => fun Heq =>
-      dispatch_aux (p :: pl, mk_let x t a) (cases,wilds)
-    | Pvar x => fun Heq =>
-      let a := mk_let x t a in
-      err_ret (union_cases pl a types cases, (pl, a) :: wilds) 
-    end eq_refl;
-  dispatch_aux (nil, a) (cases, wilds) := throw (Failure "hd").
-Next Obligation.
-unfold list_pattern_c_size; simpl.
-rewrite (pattern_c_size_unfold p), Heq. lia.
-Defined.
-Next Obligation.
-unfold list_pattern_c_size; simpl.
-rewrite (pattern_c_size_unfold p), Heq. lia.
-Defined.
-Next Obligation.
-unfold list_pattern_c_size; simpl.
-rewrite (pattern_c_size_unfold p0), Heq. lia.
-Defined. *)
-(*TODO: see how OCaml code is to see if we need Xavier trick*)
-
-Definition dispatch rl := foldr_err (fun x y => dispatch_aux' y x) rl (Mls.empty, nil) .
+Definition dispatch rl := foldr_errst dispatch_aux' (Mls.empty, nil) rl.
 
 End Dispatch.
 
+(*TODO: remove obviously*)
+Unset Guard Checking.
 (*Compile intermediate parts*)
 Section Compile.
 
@@ -203,11 +196,11 @@ Variant compile_result:=
 
 Definition compile_exn (e: errorM compile_result) : 
   errorM A :=
-  x <- e ;;
+  (x <- e ;;
   match x with
   | Succ y => err_ret y
   | NonExh ps => throw (NonExhaustive ps)
-  end.
+  end)%err.
 
 
 (*NOTE: We can have a NonExhaustive inside an OtherExn (it's all the same in
@@ -224,123 +217,261 @@ to lose the ps info (which is the whole reason we have this type)*)
   | OtherExn e => OtherExn e
   end. *)
 
-Definition comp_cases {A: Type} (compile: list term_c -> list (list pattern * A) -> errorM compile_result) 
-  cases tl ty cs al : errorM compile_result :=
-  r <- (Mls.find _ cs cases) ;;
+
+(*NOTE: CANNOT use hashcons_full because we need in decl*)
+Notation comp_res := (errState (CoqBigInt.t * hashcons_ty ty_c) compile_result).
+
+
+
+Definition comp_cases {A: Type} (compile: list term_c -> list (list pattern * A) -> comp_res)
+  cases tl ty cs al : comp_res :=
+  r <- (errst_lift2 (Mls.find _ cs cases)) ;;
   c <- compile (rev_append al tl) r ;;
   match c with
-  | Succ a => err_ret (Succ a)
+  | Succ a => errst_ret (Succ a)
   | NonExh pl => 
     (*The catch case*)
     (*We don't prove anything about this so it's fine to have a nested fix*)
     (*TODO: see if OK to use non-hashconsing-version since it's just for exception anyway*)
-    let fix cont acc vl pl : errorM (list pattern_c) := 
+    let fix cont acc vl pl : errState (CoqBigInt.t * hashcons_ty ty_c) (list pattern_c) := 
     match vl,pl with
       | (_::vl), (p::pl) => 
         cont (p::acc) vl pl
       | [], pl => 
-        p1 <- pat_app_aux cs acc ty ;;
-        err_ret (p1 :: pl)
-      | _, _ => assert_false "comp_cases failed"
+        p1 <- (errst_tup2 (pat_app cs acc ty)) ;;
+        errst_ret (p1 :: pl)
+      | _, _ => errst_lift2 (assert_false "comp_cases failed")
     end
     in
-    c <- (cont nil cs.(ls_args) pl) ;;
-    throw (NonExhaustive c)
+    c <- (cont nil cs.(ls_args) pl);;
+    errst_throw (NonExhaustive c)
+  end.
+
+Definition opt_get {A: Type} (o: option A) : errorM A :=
+  match o with
+  | Some x => err_ret x
+  | None => throw (Invalid_argument "option is None")
+  end.
+
+(*NOTE: like above, this uses unsafe functions, since we don't really care
+  about typechecking the terms we are giving back in the error message*)
+Definition comp_wilds (compile: list term_c -> list (list pattern * A) -> comp_res) 
+  (types : Mls.t (list pattern_c)) (tl : list term_c) wilds css (ty : ty_c) (_: unit) : comp_res :=
+  c <- (compile tl wilds) ;;
+  errst_tup2 (match c with
+  | Succ x => errst_ret (Succ x)
+  | NonExh pl =>
+    let find_cs cs : errorHashconsT ty_c unit :=
+      if Mls.mem _ cs types then errst_ret tt else
+      v <- errst_lift2 (opt_get cs.(ls_value)) ;;
+      tm <- ty_match Mtv.empty v ty ;;
+      let wild ty := pat_wild (ty_inst_unsafe tm ty) in
+      pw <- pat_app cs (List.map wild cs.(ls_args)) ty ;;
+      errst_throw (NonExhaustive (pw :: pl))
+    in
+    (*Cannot iter directly because we cannot include errorM in extmap due to universe
+      inconsistency*)
+    _ <- iter_errst find_cs (Sls.elements css) ;;
+    (* _ <- Sls.iter find_cs css;; *)
+    errst_throw (NonExhaustive (pat_wild ty :: pl))
+  end).
+
+
+(*And the full function*)
+(*NOTE: we don't give the termination metric or *)
+
+Variable (get_constructors: tysymbol_c -> list lsymbol) 
+  (mk_case: term_c -> list (pattern_c * A) -> errorM A)
+  (mk_let: vsymbol -> term_c -> A -> errState CoqBigInt.t A)
+  (bare: bool) (simpl_constr: bool).
+
+(*[mk_case] does not use state (t_case_close)*)
+Definition comp_full 
+  (comp_wilds: unit -> comp_res)
+  (comp_cases: lsymbol -> list term_c -> comp_res)
+  (types: Mls.t (list pattern_c)) (*tl cases wilds*) (css : Sls.t) 
+  cslist t ty (_: unit) :
+  comp_res :=
+  no_wilds <-
+    if bare then
+      t <- (errst_lift2 (Mls.choose _ types))  ;;
+      let cs := fst t in
+      errst_ret (CoqBigInt.eqb (Mls.cardinal _ types) (cs.(ls_constr)))
+    else
+      errst_ret (Mls.set_submap _ _ css types) ;;
+  base <- if (no_wilds : bool) then errst_ret []
+    else 
+      c <- comp_wilds tt ;;
+      match c with
+      | NonExh pl => errst_throw (NonExhaustive pl)
+      | Succ x =>
+          errst_ret [(pat_wild ty,x) ]
+      end ;;
+  let add (acc : list (pattern_c * A)) (x: lsymbol * list pattern_c) :
+     errState (CoqBigInt.t * hashcons_ty ty_c) (list (pattern_c * A)):=
+    (let (cs,ql) := x in
+    let get_vs q := create_vsymbol (id_fresh1 "x") (pat_ty_of q) in
+    vl <- errst_tup1 (errst_lift1 (st_list (rev_map get_vs ql))) ;;
+    let pl := rev_map pat_var vl in
+    let al := rev_map t_var vl in
+    c <- comp_cases cs al ;;
+    match c with
+    | NonExh pl => errst_throw (NonExhaustive pl)
+    | Succ x =>
+      p <- errst_tup2 (pat_app cs pl ty) ;;
+      errst_ret ((p, x) :: acc)
+    end)%errst
+  in
+  l <- (foldl_errst add cslist base) ;;
+  c <- errst_lift2 (mk_case t l) ;;
+  errst_ret (Succ c).
+
+(*TODO: Equations is awful for extraction, use wf recursion I think*)
+(*TODO: this gives terrible OCaml code*)
+Fixpoint compile_aux (tl: list term_c) (rl: list (list pattern_c * A)) { struct rl }
+  (*(ACC: Acc lt (pat_mx_size rl))*) : comp_res :=
+  match tl, rl with
+  | _, [] =>  (* no actions *)
+      pl <- errst_list (map (fun t =>
+        ty <- errst_lift2 (t_type t) ;;
+        errst_ret (pat_wild ty)) tl) ;;
+      errst_ret (NonExh pl)
+  | [], ((_, a) :: _) => errst_ret (Succ a)
+  | t :: tl, rl => (* process the leftmost column *)
+    ty <- errst_lift2 (t_type t) ;;
+    (* extract the set of constructors *)
+    let (bare,css) := match ty_node_of ty with
+      | Tyapp ts _ => if bare then (true, Sls.empty) else (false, Sls.of_list (get_constructors ts))
+          (* begin try false, Sls.of_list (get_constructors ts)
+          with Bare -> true, Sls.empty end *)
+      | Tyvar _ => (false, Sls.empty)
+      end
+    in
+    (* if bare, only check fs.ls_constr *)
+    let is_constr fs :=
+      CoqBigInt.pos fs.(ls_constr) && (bare || Sls.mem fs css)
+    in
+    (* map every constructor occurring at the head
+      * of the pattern list to the list of its args *)
+    types_cslist <- errst_lift2 (populate_all is_constr ty rl) ;;
+    let types := fst types_cslist in
+    let cslist := snd types_cslist in
+    (* dispatch every case to a primitive constructor/wild case *)
+    (*TODO: need dependent version of bind here*)
+    casewild <- errst_tup1 (dispatch mk_let t types rl) ;;
+    let cases := fst casewild in
+    let wilds := snd casewild in
+
+    (*Need to inline intermediate functions for termination*)
+
+    (*Case 1: wilds*)
+    let comp_wilds (_: unit) : comp_res :=
+      c <- (compile_aux tl wilds (*(Acc_inv ACC (size_small _ _))*)) ;;
+      errst_tup2 (match c with
+      | Succ x => errst_ret (Succ x)
+      | NonExh pl =>
+        let find_cs cs : errorHashconsT ty_c unit :=
+          if Mls.mem _ cs types then errst_ret tt else
+          v <- errst_lift2 (opt_get cs.(ls_value)) ;;
+          tm <- ty_match Mtv.empty v ty ;;
+          let wild ty := pat_wild (ty_inst_unsafe tm ty) in
+          pw <- pat_app cs (List.map wild cs.(ls_args)) ty ;;
+          errst_throw (NonExhaustive (pw :: pl))
+        in
+        (*Cannot iter directly because we cannot include errorM in extmap due to universe
+          inconsistency*)
+        _ <- iter_errst find_cs (Sls.elements css) ;;
+        (* _ <- Sls.iter find_cs css;; *)
+        errst_throw (NonExhaustive (pat_wild ty :: pl))
+      end)
+    in
+
+    (* how to proceed if [t] is [Tapp(cs,al)] and [cs] is in [cases] *)
+    let comp_cases cs al : comp_res := 
+      r <- (errst_lift2 (Mls.find _ cs cases)) ;;
+      c <- compile_aux (rev_append al tl) r (*(Acc_inv ACC (size_small _ _)*) ;;
+      match c with
+      | Succ a => errst_ret (Succ a)
+      | NonExh pl => 
+        (*The catch case*)
+        (*We don't prove anything about this so it's fine to have a nested fix*)
+        (*TODO: see if OK to use non-hashconsing-version since it's just for exception anyway*)
+        let fix cont acc vl pl : errState (CoqBigInt.t * hashcons_ty ty_c) (list pattern_c) := 
+        match vl,pl with
+          | (_::vl), (p::pl) => 
+            cont (p::acc) vl pl
+          | [], pl => 
+            p1 <- (errst_tup2 (pat_app cs acc ty)) ;;
+            errst_ret (p1 :: pl)
+          | _, _ => errst_lift2 (assert_false "comp_cases failed")
+        end
+        in
+        c <- (cont nil cs.(ls_args) pl);;
+        errst_throw (NonExhaustive c)
+      end
+    in
+    
+    (* how to proceed if [t] is not covered by [cases] *)
+    (*comp_full above*)
+
+    (* assemble the primitive case statement *)
+    if Mls.is_empty _ types then
+      comp_wilds tt
+    else if simpl_constr then
+      match t_node_of t with
+      (* | _ when Mls.is_empty types ->
+          comp_wilds () *)
+      | Tapp cs al => if is_constr cs then
+          if Mls.mem _ cs types then comp_cases cs al else 
+            comp_wilds tt
+          else comp_full comp_wilds comp_cases types css cslist t ty tt
+      | _ => comp_full comp_wilds comp_cases types css cslist t ty tt
+          
+        end
+      else comp_full comp_wilds comp_cases types css cslist t ty tt
+  end.
+
+Definition compile_aux' (tl: list term_c) (rl: list (list pattern_c * A))
+  (*(ACC: Acc lt (pat_mx_size rl))*) : errState (CoqBigInt.t * hashcons_ty ty_c) A :=
+  x <- compile_aux tl rl ;;
+  match x with
+  | Succ x => errst_ret x
+  | NonExh pl => errst_throw (NonExhaustive pl)
   end.
 
 End Compile.
 
+Set Guard Checking.
 
-(*TODO: let's see*)
-(*TODO: Equations*)
-(*Unlike their exception method, we will use an extra "bare" param*)
-(*Section Compile.
-Context {A: Type} (get_constructors: tysymbol_c -> list lsymbol) 
-  (mk_case: term_c -> list (pattern * A) -> A) 
-  (mk_let: vsymbol -> term_c -> A -> A).
-Fixpoint compile_aux (bare: bool) 
-  (tl: list term_c) (rl: list (list pattern_c * A)): errorM A :=
-  match tl, rl with
-  | _, nil => 
-    pl1 <- errorM_list (map t_type tl) ;;
-    let pl := map pat_wild pl1 in
-    throw (NonExhaustive pl)
-  | nil, (_ , a) :: _ => err_ret a
-  | t :: tl, _ =>
-    ty <- t_type t ;;
-    (*Extract the set of constructors*)
-    let (bare, css) := match ty_node_of ty with
-      | Tyapp ts _ =>
-        if bare then (true, Sls.empty) else
-        (false, Sls.of_list (get_constructors ts))
-      | Tyvar _ => (false,  Sls.empty)
-    end
-    in
-    (*if bare, only check fs.ls_constr*)
-    let is_constr fs :=
-      CoqBigInt.lt CoqBigInt.zero (fs.(ls_constr)) &&
-        (bare || Sls.mem fs css)
-    in
-    (*map every constructor ocurring at the head of the pattern list
-      to the list of its args*)
-    types_cslist <- 
-      let fix populate acc p : errorM (Mls.t (list pattern_c) * list (lsymbol * list pattern_c)) :=
-        match pat_node_of p with
-        | Pwild => err_ret acc
-        | Pvar _ => err_ret acc
-        | Pas p _ => populate acc p
-        | Por p q =>
-          p1 <- (populate acc p);; 
-          populate p1 q
-        | Papp fs pl =>
-          if is_constr fs then
-            if Mls.mem _ fs (fst acc) then err_ret acc else
-            err_ret (Mls.add fs pl (fst acc), ((fs, pl) :: (snd acc)))
-          else throw (ConstructorExpected (fs, ty))
-        end
-        in
-      let populate acc (x: list pattern_c * A) : 
-        errorM (Mls.t (list pattern_c) * list (lsymbol * list pattern_c))  := 
-        p <- hd (fst x) ;;
-        populate acc p in
-      foldl_err populate rl (Mls.empty, nil)
-    ;;
-    let types := fst types_cslist in
-    let cslist := snd types_cslist in
-    (*dispatch every case to a primitive constructor/wild case*)
-    let cases_wilds :=
-      let add_case fs ls a cases :=
-        Mls.change (fun x =>
-          match x with
-          | None => Some [(pl, a)]
-          | Some rl => Some ((pl, a) :: rl)
-          end) fs cases
-      in
-      let union_cases pl a types cases :=
-        let add pl q := pat_wild (pat_ty_of q) :: pl in
-        let wild ql := [(fold_left add pl ql, a)] in
-        let join _ wl rl := Some (wl ++ rl) in
-        Mls.union join (Mls.map wild types) cases
-      in
-      let rec dispatch (pla: list pattern * A) casewild :=
-        let cases := fst casewild in
-        let wilds := snd casewild in
-        p <- hd (fst pla) ;;
-        pl <- tl (fst pla) ;;
-        match (pat_node_of p) with
-        | Papp fs pl' =>
-          (add_case fs (rev_append pl' pl) a cases, wilds)
-        | Pwild => (union_cases pl a types cases, (pl, a) :: wilds)
-        | Por p1 q1 =>
-          d1 <- dispatch (q :: pl, a) (cases, wilds) ;;
-          dispatch (p :: pl, a) d1
-        | Pas p x =>
-          dispatch (p :: pl, mk_let x t a) (cases_wilds)
-        | Pvar x => 
-          let a := mk_let x t a in
-          union_cases pl a types cases 
+(*The derived functions (NOTE: ours are "aux" because we don't have named arguments)*)
+Definition compile_bare_aux {A: Type} mk_case mk_let tl (rl : list (list pattern_c * A)) :=
+  let get_constructors _ := nil in
+  x <- compile_aux get_constructors mk_case mk_let true true tl rl ;;
+  match x with
+  | Succ x => errst_ret x
+  | NonExh pl => errst_throw (NonExhaustive nil) (*NOTE: not exactly the same, since
+    we could have thrown an error before*)
+  end.
 
-          (*TODO: do in many parts, add each individually*)
+Definition check_compile_aux get_constructors tl (ps: list (list pattern_c)) :
+  errState (CoqBigInt.t * hashcons_ty ty_c) unit :=
+  match ps with
+  | nil => 
+    pl <- (errst_list (map (fun t => 
+      ty <- errst_lift2 (t_type t) ;;
+      errst_ret (pat_wild ty)) tl)) ;;
+    errst_throw (NonExhaustive pl)
+  | pl :: _ =>
+    let mkt p := 
+      i <- errst_lift1 (create_vsymbol (id_fresh1 "_") (pat_ty_of p)) ;;
+      errst_ret (t_var i) in
+    tl <- if null tl then 
+      errst_tup1 (errst_list (map mkt pl)) else errst_ret tl ;;
+    let rl := map (fun pl => (pl, t_true)) ps in
+    let mk_case := t_case_close in
+    let mk_let := t_let_close_simp in (*NOTE: cannot use unit because of proofs*)
+    (*let mk_case _ _ := tt and mk_let _ _ _ := tt in (*TODO: change this*)*)
+    _ <- compile_aux get_constructors mk_case mk_let false false tl rl;;
+    errst_ret tt
+  end.
 
-     throw (NonExhaustive nil)
-  end. *)
